isabelle/Chapter13_4_Evaluation.thy
@@ -2,6 +2,111 @@ theory Chapter13_4_Evaluation
 imports Chapter13_3_PatternMatching
 begin
 
+
+inductive extract_constraint :: "patn => type => constr => bool"       
+where [simp]: "extract_constraint Wild t All"
+    | [simp]: "extract_constraint PVar t All"
+    | [simp]: "extract_constraint PTriv Unit CTriv"
+    | [simp]: "extract_constraint p1 t1 c1 ==> extract_constraint p2 t2 c2 ==> extract_constraint (PPair p1 p2) (Prod t1 t2) (CPair c1 c2)"
+    | [simp]: "extract_constraint p t1 c ==> extract_constraint (PInL p) (Sum t1 t2) (CInL t1 t2 c)"
+    | [simp]: "extract_constraint p t2 c ==> extract_constraint (PInR p) (Sum t1 t2) (CInR t1 t2 c)"
+ 
+inductive_cases [elim!]: "extract_constraint Wild t c"
+inductive_cases [elim!]: "extract_constraint PVar t c"
+inductive_cases [elim!]: "extract_constraint PTriv t c"
+inductive_cases [elim!]: "extract_constraint (PPair p1 p2) t c"
+inductive_cases [elim!]: "extract_constraint (PInL p) t c"
+inductive_cases [elim!]: "extract_constraint (PInR p) t c"
+
+lemma [simp]: "extract_constraint PTriv Unit c ==> c = CTriv"
+by (induction PTriv Unit c rule: extract_constraint.induct, simp)
+
+lemma [simp]: "extract_constraint (PPair p1 p2) (Prod t1 t2) c ==> 
+      EX c1 c2. extract_constraint p1 t1 c1 & extract_constraint p2 t2 c2 & c = CPair c1 c2"
+by (induction "PPair p1 p2" "Prod t1 t2" c rule: extract_constraint.induct, simp)
+
+lemma [simp]: "extract_constraint (PInL p) (Sum t1 t2) c ==> 
+      EX c'. extract_constraint p t1 c' & c = CInL t1 t2 c'"
+by (induction "PInL p" "Sum t1 t2" c rule: extract_constraint.induct, simp)
+
+lemma [simp]: "extract_constraint (PInR p) (Sum t1 t2) c ==> 
+      EX c'. extract_constraint p t2 c' & c = CInR t1 t2 c'"
+by (induction "PInR p" "Sum t1 t2" c rule: extract_constraint.induct, simp)
+
+inductive all_matches_complete :: "expr => type => bool"
+      and extract_constraints :: "rule list => type => constr => bool"
+      and extract_constraint_rule :: "rule => type => constr => bool"
+where [simp]: "all_matches_complete (Var v) t" 
+    | [simp]: "all_matches_complete Zero Nat"
+    | [simp]: "all_matches_complete e Nat ==> all_matches_complete (Succ e) Nat"
+    | [simp]: "all_matches_complete e1 t ==> all_matches_complete e2 t ==> all_matches_complete e3 Nat ==> all_matches_complete (IsZ e1 e2 e3) t"
+    | [simp]: "all_matches_complete e (Arr t' t) ==> all_matches_complete (Lam t' e) t"
+    | [simp]: "all_matches_complete e1 (Arr t' t) ==> all_matches_complete e2 t' ==> all_matches_complete (Ap e1 e2) t" (* t' *)
+    | [simp]: "all_matches_complete e t ==> all_matches_complete (Fix t e) t"
+    | [simp]: "all_matches_complete Triv Unit"
+    | [simp]: "all_matches_complete e1 t1 ==> all_matches_complete e2 t2 ==> all_matches_complete (Pair e1 e2) (Prod t1 t2)"
+    | [simp]: "all_matches_complete e (Prod t1 t2) ==> all_matches_complete (ProjL e) t1" (* t2 *)
+    | [simp]: "all_matches_complete e (Prod t1 t2) ==> all_matches_complete (ProjR e) t2" (* t1 *)
+    | [simp]: "all_matches_complete e Void ==> all_matches_complete (Abort t e) t"
+    | [simp]: "all_matches_complete e t1 ==> all_matches_complete (InL t1 t2 e) (Sum t1 t2)"
+    | [simp]: "all_matches_complete e t2 ==> all_matches_complete (InR t1 t2 e) (Sum t1 t2)"
+    | [simp]: "all_matches_complete e t' ==> extract_constraints rs t' c ==> totally_satisfied t' c ==> all_matches_complete (Match e rs) t" (* t' *)
+    | [simp]: "extract_constraints [] t Nothing"
+    | [simp]: "extract_constraint_rule r t c1 ==> extract_constraints rs t c2 ==> extract_constraints (r # rs) t (Or c1 c2)"
+    | [simp]: "extract_constraint p t c ==> all_matches_complete e t ==> extract_constraint_rule (Rule p e) t c"
+
+inductive_cases [elim!]: "all_matches_complete (Var x) t"
+inductive_cases [elim!]: "all_matches_complete Zero t"
+inductive_cases [elim!]: "all_matches_complete (Succ x) t"
+inductive_cases [elim!]: "all_matches_complete (IsZ x y z) t"
+inductive_cases [elim!]: "all_matches_complete (Lam x y) t"
+inductive_cases [elim!]: "all_matches_complete (Ap x y) t"
+inductive_cases [elim!]: "all_matches_complete (Fix x y) t"
+inductive_cases [elim!]: "all_matches_complete Triv t"
+inductive_cases [elim!]: "all_matches_complete (Pair x y) t"
+inductive_cases [elim!]: "all_matches_complete (ProjL v) t"
+inductive_cases [elim!]: "all_matches_complete (ProjR v) t"
+inductive_cases [elim!]: "all_matches_complete (Abort x y) t"
+inductive_cases [elim!]: "all_matches_complete (InL x y z) t"
+inductive_cases [elim!]: "all_matches_complete (InR x y z) t"
+inductive_cases [elim!]: "all_matches_complete (Match x y) t"
+inductive_cases [elim!]: "extract_constraints [] t c"
+inductive_cases [elim!]: "extract_constraints (x # y) t c"
+inductive_cases [elim!]: "extract_constraint_rule (Rule x y) t c"
+
+lemma [simp]: "types_from_pat p t ts ==> extract_constraint p t c ==> satisfies e c ==> EX s. matches s p e"
+proof (induction p t ts arbitrary: e rule: types_from_pat.induct)
+case tpwld
+  have "matches [] Wild e" by simp
+  thus ?case by (rule exI)
+next case tpvar
+  have "matches [e] PVar e" by simp
+  thus ?case by (rule exI)
+next case tptrv
+  hence "c = CTriv" by simp
+  with tptrv have X: "e = Triv" by simp
+  have "matches [] PTriv Triv" by simp
+  hence "EX s. matches s PTriv Triv" by (rule exI)
+  with X show ?case by simp
+next case (tppar p1 t1 _ p2 t2 _)
+  hence "EX c1 c2. extract_constraint p1 t1 c1 & extract_constraint p2 t2 c2 & c = CPair c1 c2" by auto
+  with tppar show ?case
+  proof auto
+    fix e1 e2 c1 c2
+    assume "extract_constraint p1 t1 c1"
+       and "extract_constraint p2 t2 c2"
+       and "!!ee. extract_constraint p1 t1 (CPair c1 c2) \<Longrightarrow> satisfies ee (CPair c1 c2) \<Longrightarrow> \<exists>s. matches s p1 ee"
+       and "!!ee. extract_constraint p2 t2 (CPair c1 c2) \<Longrightarrow> satisfies ee (CPair c1 c2) \<Longrightarrow> \<exists>s. matches s p2 ee"
+       and "satisfies e1 c1" 
+       and "satisfies e2 c2"
+    show "EX s. matches s (PPair p1 p2) (Pair e1 e2)" by simp sorry
+  qed
+next case (tpinl p t1 _ t2)
+  thus ?case by simp sorry
+next case (tpinr p t2 _ t1)
+  thus ?case by simp sorry
+qed
+
 inductive eval :: "expr => expr => bool"
 where esuc [simp]: "eval n n' ==> eval (Succ n) (Succ n')"
     | eap1 [simp]: "eval e1 e1' ==> eval (Ap e1 e2) (Ap e1' e2)"
@@ -24,19 +129,19 @@ where esuc [simp]: "eval n n' ==> eval (Succ n) (Succ n')"
     | emt2 [simp]: "is_val e ==> matches s p e ==> eval (Match e (Rule p e2 # rs)) (apply_subst s e2)"
     | emt3 [simp]: "is_val e ==> no_match e p ==> eval (Match e rs) e' ==> eval (Match e (Rule p e2 # rs)) e'"
 
-theorem preservation: "eval e e' ==> typecheck env e t ==> all_matches_complete e t ==> typecheck env e' t"
+theorem preservation: "eval e e' ==> typecheck env e t ==> typecheck env e' t"
 proof (induction e e' arbitrary: t env rule: eval.induct)
 case esuc
   thus ?case by auto
 next case (eap1 e1 e1' e2)
-  hence "EX t2. typecheck env e1' (Arr t2 t) & typecheck env e2 t2" by auto sorry
+  hence "EX t2. typecheck env e1' (Arr t2 t) & typecheck env e2 t2" by auto
   thus ?case by auto
-next case eap2
-  thus ?case by auto sorry
+next case (eap2 e1 e2 e2')
+  thus ?case by auto
 next case eap3
   thus ?case by auto
 next case eiz1
-  thus ?case by auto sorry
+  thus ?case by auto
 next case eiz2
   thus ?case by auto
 next case eiz3
@@ -44,27 +149,27 @@ next case eiz3
 next case efix
   thus ?case by auto
 next case epa1
-  thus ?case by auto sorry
+  thus ?case by auto
 next case epa2
-  thus ?case by auto sorry
+  thus ?case by auto
 next case (epl1 e e')
-  hence "!!t2. typecheck env e (Prod t t2) ==> typecheck env e' (Prod t t2)" by simp sorry
+  hence "!!t2. typecheck env e (Prod t t2) ==> typecheck env e' (Prod t t2)" by simp
   with epl1 have "EX t2. typecheck env e' (Prod t t2)" by auto
   thus ?case by auto
 next case epl2
   thus ?case by auto
 next case (epr1 e e')
-  hence "!!t1. typecheck env e (Prod t1 t) ==> typecheck env e' (Prod t1 t)" by simp sorry
+  hence "!!t1. typecheck env e (Prod t1 t) ==> typecheck env e' (Prod t1 t)" by simp
   with epr1 have "EX t1. typecheck env e' (Prod t1 t)" by auto
   thus ?case by auto
 next case epr2
   thus ?case by auto
 next case eabt
-  thus ?case by auto sorry
+  thus ?case by auto
 next case einl
-  thus ?case by auto sorry
+  thus ?case by auto
 next case einr
-  thus ?case by auto sorry
+  thus ?case by auto
 next case (emt1 e e' rs)
   hence "EX t1. typecheck env e t1 & typecheck_rules env rs t1 t" by auto
   thus ?case
@@ -72,7 +177,7 @@ next case (emt1 e e' rs)
     fix t1 c
     assume "typecheck env e t1"
        and "typecheck_rules env rs t1 t"
-    moreover with emt1 have "typecheck env e' t1" by simp sorry
+    moreover with emt1 have "typecheck env e' t1" by simp
     ultimately show "typecheck env (Match e' rs) t" by simp
   qed
 next case (emt2 e s p e' rs)
@@ -95,30 +200,12 @@ next case (emt2 e s p e' rs)
       ultimately show "typecheck_subst env s ts" by simp
     qed
     with X show "typecheck env (apply_subst s e') t" by simp
-  next 
-    fix t1 ts
-    assume W: "is_val e" 
-       and V: "matches s p e" 
-       and Z: "typecheck env e t1" 
-       and Y: "types_from_pat p t1 ts" 
-       and X: "typecheck (extend_env ts env) e' t" 
-    have "types_from_pat p t1 ts ==> typecheck env e t1 ==> is_val e ==> (EX s. typecheck_subst env s ts & matches s p e) | no_match e p" by simp
-    with Y Z W V have "EX s. typecheck_subst env s ts & matches s p e" by simp
-    hence "typecheck_subst env s ts"
-    proof auto
-      fix sa
-      assume "typecheck_subst env sa ts" 
-         and "matches sa p e"
-      moreover with V have "sa = s" by simp 
-      ultimately show "typecheck_subst env s ts" by simp
-    qed
-    with X show "typecheck env (apply_subst s e') t" by simp
   qed
 next case (emt3 e p rs e' e2)
-  thus ?case by auto sorry
+  thus ?case by auto
 qed
 
-theorem progress: "typecheck env e t ==> env = empty_map ==> is_val e | (EX e'. eval e e')"
+theorem progress: "typecheck env e t ==> env = empty_map ==> all_matches_complete e t ==> is_val e | (EX e'. eval e e')"
     and "typecheck_rules env rs t1 t ==> env = empty_map ==> True"
     and "typecheck_rule env r t1 t ==> env = empty_map ==> True"
 proof (induction env e t rule: typecheck_typecheck_rules_typecheck_rule.inducts)
@@ -157,7 +244,7 @@ next case (trec env e e0 t e1)
     qed
     thus ?thesis by simp
   next case False
-    with trec have "\<exists>a. eval e a" by simp
+    with trec have "\<exists>a. eval e a" by auto
     thus ?thesis
     proof auto
       fix a
@@ -171,7 +258,7 @@ next case tlam
 next case (tapp env e1 t2 t e2)
   from tapp have "typecheck env e1 (Arr t2 t)" by simp
   from tapp have "typecheck env e2 t2" by simp
-  from tapp have "is_val e2 \<or> (\<exists>a. eval e2 a)" by simp
+  from tapp have "is_val e2 \<or> (\<exists>a. eval e2 a)" by auto sorry
   thus ?case
   proof (cases "is_val e1")
   case True
@@ -188,7 +275,7 @@ next case (tapp env e1 t2 t e2)
         thus "EX x. eval (Ap (Lam t2 v) e2) x" by auto
       qed
     next case False
-      with tapp have "\<exists>a. eval e2 a" by simp
+      with tapp have "\<exists>a. eval e2 a" by auto sorry
       thus ?thesis
       proof auto
         fix a
@@ -199,7 +286,7 @@ next case (tapp env e1 t2 t e2)
       qed
     qed
   next case False
-    with tapp have "\<exists>a. eval e1 a" by simp
+    with tapp have "\<exists>a. eval e1 a" by auto sorry
     thus ?thesis
     proof auto
       fix a
@@ -224,7 +311,7 @@ next case (tpar env e1 t1 e2 t2)
     case True
       with X show ?thesis by simp  
     next case False
-      with tpar have "EX a. eval e2 a" by simp
+      with tpar have "EX a. eval e2 a" by auto
       hence "EX a. eval (Pair e1 e2) a"
       proof auto
         fix e2'
@@ -235,7 +322,7 @@ next case (tpar env e1 t1 e2 t2)
       thus ?thesis by simp  
     qed
   next case False
-    with tpar have "EX a. eval e1 a" by simp
+    with tpar have "EX a. eval e1 a" by auto
     hence "EX a. eval (Pair e1 e2) a"
     proof auto
       fix e1'
@@ -259,7 +346,7 @@ next case (tprl env e t1 t2)
       thus "EX a. eval (ProjL (Pair e1 e2)) a" by auto
     qed
   next case False
-    with tprl have "EX a. eval e a" by simp
+    with tprl have "EX a. eval e a" by auto sorry
     thus ?thesis
     proof auto
       fix a
@@ -282,7 +369,7 @@ next case (tprr env e t1 t2)
       thus "EX a. eval (ProjR (Pair e1 e2)) a" by auto
     qed
   next case False
-    with tprr have "EX a. eval e a" by simp
+    with tprr have "EX a. eval e a" by auto sorry
     thus ?thesis
     proof auto
       fix a
@@ -323,10 +410,10 @@ next case (tmch env e t1 rs t2)
     from tmch have "typecheck env e t1" by simp
     from tmch have "typecheck_rules env rs t1 t2" by simp
 
-    hence "EX a. eval (Match e rs) a" by simp sorry
+    hence "EX a. eval (Match e rs) a" by auto sorry
     thus ?thesis by simp
   next case False
-    with tmch have "EX a. eval e a" by simp
+    with tmch have "EX a. eval e a" by auto sorry
     thus ?thesis
     proof auto
       fix a
